Coq/Cln/Cln_CompositeExcursion.v
@@ -1,0 +1,507 @@
+(*
+  ============================================================
+  File: Cln_CompositeExcursion.v
+  ============================================================
+*)
+
+Require Import Cln_Full.
+Require Import Cln_Grade.
+Require Import Cln_finite_l1_submultiplicativity.
+Require Import Cln_BoolDist.
+
+From Coq Require Import List Lia Arith.
+From Coq Require Import QArith.
+From Coq Require Import QArith.QArith_base.
+From Coq Require Import QArith.Qabs.
+From Coq Require Import Bool.
+
+Import ListNotations.
+Open Scope Q_scope.
+Set Implicit Arguments.
+
+Definition Qmax (a b : Q) : Q :=
+  if Qle_bool a b then b else a.
+
+Lemma Qmax_l : forall a b, a <= Qmax a b.
+Proof.
+  intros a b.
+  unfold Qmax.
+  destruct (Qle_bool a b) eqn:H.
+  - apply Qle_bool_iff in H. exact H.
+  - apply Qle_refl.
+Qed.
+
+Lemma Qmax_r : forall a b, b <= Qmax a b.
+Proof.
+  intros a b; unfold Qmax.
+  destruct (Qle_bool a b) eqn:H.
+  - apply Qle_refl.
+  -
+    assert (Hnot : ~(a <= b)).
+    { intro Hab.
+      apply (proj2 (Qle_bool_iff a b)) in Hab.
+      rewrite Hab in H; discriminate.
+    }
+    destruct (Qcompare_spec b a) as [Hc | Hc | Hc].
+    all: try (
+      apply Qlt_le_weak; exact Hc
+    ).
+    all: try (
+      rewrite Hc; apply Qle_refl
+    ).
+    exfalso.
+    apply Hnot.
+    apply Qlt_le_weak.
+    exact Hc.
+Qed.
+
+Fixpoint list_Qmax (xs : list Q) : Q :=
+  match xs with
+  | [] => 0
+  | x :: tl => Qmax x (list_Qmax tl)
+  end.
+
+Fixpoint max_l1_during {n} (sq : Vector.t Q n) (e : GA_expr n) : Q :=
+  match e with
+  | Basis _   => 1
+  | Scalar c  => Qabs c
+  | Cln_Grade.Add e1 e2 =>
+      max_l1_during sq e1 + max_l1_during sq e2
+  | Mul e1 e2 =>
+      Qmax (Qmax (max_l1_during sq e1) (max_l1_during sq e2))
+           (l1_norm (mv_gp sq (eval_expr sq e1) (eval_expr sq e2)))
+  | Conv e1 e2 =>
+      Qmax (Qmax (max_l1_during sq e1) (max_l1_during sq e2))
+           (l1_norm (mv_conv (eval_expr sq e1) (eval_expr sq e2)))
+  end.
+
+Lemma l1_eval_le_max_l1_during :
+  forall n (sq : Vector.t Q n) (e : GA_expr n),
+    l1_norm (eval_expr sq e) <= max_l1_during sq e.
+Proof.
+  intros n sq e.
+  induction e as [i|c|e1 IH1 e2 IH2|e1 IH1 e2 IH2|e1 IH1 e2 IH2]; simpl.
+  - apply Qle_of_Qeq. apply l1_norm_basis.
+  - apply Qle_of_Qeq. apply l1_norm_scale_one.
+  -
+    eapply Qle_trans.
+    + apply l1_add_bound.
+    +
+      apply Qplus_le_compat; assumption.
+  - apply Qmax_r.
+  - apply Qmax_r.
+Qed.
+
+Definition dist_to {n} (F : MV n) (f : Corner n -> bool) : Q :=
+  bool_dist_wrt F f.
+
+Definition boolish_le {n} (F : MV n) (d : Q) : Prop :=
+  exists g : Corner n -> bool, bool_dist_wrt F g <= d.
+
+Fixpoint max_booldist_during {n}
+  (sq : Vector.t Q n)
+  (f  : Corner n -> bool)
+  (e  : GA_expr n) : Q :=
+  match e with
+  | Basis _  => dist_to (eval_expr sq e) f
+  | Scalar _ => dist_to (eval_expr sq e) f
+  | Cln_Grade.Add e1 e2 =>
+      Qmax
+        (Qmax (max_booldist_during sq f e1)
+              (max_booldist_during sq f e2))
+        (dist_to (eval_expr sq (Cln_Grade.Add e1 e2)) f)
+  | Mul e1 e2 =>
+      Qmax
+        (Qmax (max_booldist_during sq f e1)
+              (max_booldist_during sq f e2))
+        (dist_to (mv_gp sq (eval_expr sq e1) (eval_expr sq e2)) f)
+  | Conv e1 e2 =>
+      Qmax
+        (Qmax (max_booldist_during sq f e1)
+              (max_booldist_during sq f e2))
+        (dist_to (mv_conv (eval_expr sq e1) (eval_expr sq e2)) f)
+  end.
+
+Lemma booldist_eval_le_max_booldist_during :
+  forall n (sq : Vector.t Q n) (f : Corner n -> bool) (e : GA_expr n),
+    dist_to (eval_expr sq e) f <= max_booldist_during sq f e.
+Proof.
+  intros n sq f e.
+  induction e as [i|c|e1 IH1 e2 IH2|e1 IH1 e2 IH2|e1 IH1 e2 IH2]; simpl.
+  - apply Qle_refl.
+  - apply Qle_refl.
+  - (* Add *) apply Qmax_r.
+  - (* Mul *) apply Qmax_r.
+  - (* Conv *) apply Qmax_r.
+Qed.
+
+Fixpoint trace_boolish_le {n} (sq : Vector.t Q n) (e : GA_expr n) (d : Q) : Prop :=
+  match e with
+  | Basis _ | Scalar _ => boolish_le (eval_expr sq e) d
+  | Cln_Grade.Add e1 e2 =>
+      trace_boolish_le sq e1 d /\ trace_boolish_le sq e2 d /\
+      boolish_le (eval_expr sq (Cln_Grade.Add e1 e2)) d
+  | Mul e1 e2 =>
+      trace_boolish_le sq e1 d /\ trace_boolish_le sq e2 d /\
+      boolish_le (mv_gp sq (eval_expr sq e1) (eval_expr sq e2)) d
+  | Conv e1 e2 =>
+      trace_boolish_le sq e1 d /\ trace_boolish_le sq e2 d /\
+      boolish_le (mv_conv (eval_expr sq e1) (eval_expr sq e2)) d
+  end.
+
+Record ExcNum := {
+  exc_grade : nat;
+  exc_l1    : Q;
+}.
+
+Definition exc_of {n} (sq : Vector.t Q n) (e : GA_expr n) : ExcNum :=
+  {| exc_grade := max_grade_during sq e;
+     exc_l1    := max_l1_during sq e |}.
+
+Definition exc_le (a b : ExcNum) : Prop :=
+  (exc_grade a < exc_grade b)%nat \/
+  (exc_grade a = exc_grade b /\ exc_l1 a < exc_l1 b) \/
+  (exc_grade a = exc_grade b /\ exc_l1 a == exc_l1 b).
+
+Definition exc_pre (a b : ExcNum) : Prop :=
+  (exc_grade a <= exc_grade b)%nat /\ exc_l1 a <= exc_l1 b.
+
+Definition computes {n} (sq : Vector.t Q n) (e : GA_expr n) (f : Corner n -> bool) : Prop :=
+  forall m : Mask n, eval_expr sq e m == embed f m.
+
+Fixpoint expr_size {n} (e : GA_expr n) : nat :=
+  match e with
+  | Basis _ => 1
+  | Scalar _ => 1
+  | Cln_Grade.Add e1 e2 => 1 + expr_size e1 + expr_size e2
+  | Mul e1 e2 => 1 + expr_size e1 + expr_size e2
+  | Conv e1 e2 => 1 + expr_size e1 + expr_size e2
+  end.
+
+Definition easy_under
+  (B : nat -> ExcNum) (d : Q)
+  {n} (sq : Vector.t Q n) (f : Corner n -> bool) : Prop :=
+  exists e : GA_expr n,
+    computes sq e f /\
+    exc_pre (exc_of sq e) (B (expr_size e)) /\
+    trace_boolish_le sq e d.
+
+Definition hard_under
+  (B : nat -> ExcNum) (d : Q)
+  {n} (sq : Vector.t Q n) (f : Corner n -> bool) : Prop :=
+  forall e : GA_expr n,
+    computes sq e f ->
+    ~ (exc_pre (exc_of sq e) (B (expr_size e)) /\ trace_boolish_le sq e d).
+
+Lemma exc_pre_refl : forall a, exc_pre a a.
+Proof.
+  intro a; split; [lia | apply Qle_refl].
+Qed.
+
+Lemma exc_pre_trans : forall a b c,
+  exc_pre a b -> exc_pre b c -> exc_pre a c.
+Proof.
+  intros a b c Hab Hbc.
+  destruct Hab as [Hg1 Hl1].
+  destruct Hbc as [Hg2 Hl2].
+  repeat split.
+  - lia.
+  - eapply Qle_trans; eauto.
+Qed.
+
+Definition exc_score (E : ExcNum) : Q :=
+  (inject_Z (Z.of_nat (exc_grade E))) + exc_l1 E.
+
+Parameter proj_bool : forall n, MV n -> Corner n -> bool.
+
+Definition represents {n} (sq : Vector.t Q n) (e : GA_expr n) (f : Corner n -> bool) : Prop :=
+  forall x : Corner n, proj_bool (eval_expr sq e) x = f x.
+
+Definition looks_hard (B : nat -> ExcNum) (d : Q) {n} (sq : Vector.t Q n) (f : Corner n -> bool) : Prop :=
+  exists e : GA_expr n,
+    computes sq e f /\
+    ~ (exc_pre (exc_of sq e) (B (expr_size e)) /\ trace_boolish_le sq e d).
+
+Lemma dist_to_unfold :
+  forall n (F : MV n) (f : Corner n -> bool),
+    dist_to F f == l1_norm (mv_sub F (embed f)).
+Proof. intros; reflexivity. Qed.
+
+(* Every correct program ends with BoolDist == 0 *)
+Lemma computes_implies_final_booldist_zero :
+  forall n (sq : Vector.t Q n) (e : GA_expr n) (f : Corner n -> bool),
+    computes sq e f ->
+    dist_to (eval_expr sq e) f == 0.
+Proof.
+  intros n sq e f Hcomp.
+  unfold dist_to, bool_dist_wrt.
+  assert (Hext :
+    l1_norm (mv_sub (eval_expr sq e) (embed f)) == l1_norm (@mv_zero n)).
+  { apply l1_norm_ext.
+    intro m.
+    unfold mv_sub, mv_zero.
+    specialize (Hcomp m).
+    rewrite Hcomp.
+    ring.
+  }
+  eapply Qeq_trans.
+  - exact Hext.
+  -
+    unfold l1_norm, mv_zero.
+    eapply Qeq_trans.
+    + apply sumQ_map_ext. intros m _.
+      rewrite Qabs_pos; [reflexivity | apply Qle_refl].
+    + apply sumQ_map_const0.
+Qed.
+
+Lemma trace_boolish_le_sub_left :
+  forall n (sq : Vector.t Q n) (d : Q) (e1 e2 : GA_expr n),
+    trace_boolish_le sq (Cln_Grade.Add e1 e2) d -> trace_boolish_le sq e1 d.
+Proof.
+  intros n sq d e1 e2 H.
+  simpl in H.
+  tauto.
+Qed.
+
+Lemma trace_boolish_le_sub_right_Add :
+  forall n (sq : Vector.t Q n) (d : Q) (e1 e2 : GA_expr n),
+    trace_boolish_le sq (Cln_Grade.Add e1 e2) d ->
+    trace_boolish_le sq e2 d.
+Proof.
+  intros n sq d e1 e2 H.
+  simpl in H.
+  tauto.
+Qed.
+
+Lemma trace_boolish_le_sub_left_Mul :
+  forall n (sq : Vector.t Q n) (d : Q) (e1 e2 : GA_expr n),
+    trace_boolish_le sq (Mul e1 e2) d ->
+    trace_boolish_le sq e1 d.
+Proof.
+  intros n sq d e1 e2 H.
+  simpl in H.
+  tauto.
+Qed.
+
+Lemma trace_boolish_le_sub_right_Mul :
+  forall n (sq : Vector.t Q n) (d : Q) (e1 e2 : GA_expr n),
+    trace_boolish_le sq (Mul e1 e2) d ->
+    trace_boolish_le sq e2 d.
+Proof.
+  intros n sq d e1 e2 H.
+  simpl in H.
+  tauto.
+Qed.
+
+Lemma trace_boolish_le_sub_left_Conv :
+  forall n (sq : Vector.t Q n) (d : Q) (e1 e2 : GA_expr n),
+    trace_boolish_le sq (Conv e1 e2) d ->
+    trace_boolish_le sq e1 d.
+Proof.
+  intros n sq d e1 e2 H.
+  simpl in H.
+  tauto.
+Qed.
+
+Lemma trace_boolish_le_sub_right_Conv :
+  forall n (sq : Vector.t Q n) (d : Q) (e1 e2 : GA_expr n),
+    trace_boolish_le sq (Conv e1 e2) d ->
+    trace_boolish_le sq e2 d.
+Proof.
+  intros n sq d e1 e2 H.
+  simpl in H.
+  tauto.
+Qed.
+
+Lemma trace_boolish_le_node_Add :
+  forall n (sq : Vector.t Q n) (d : Q) (e1 e2 : GA_expr n),
+    trace_boolish_le sq (Cln_Grade.Add e1 e2) d ->
+    boolish_le (eval_expr sq (Cln_Grade.Add e1 e2)) d.
+Proof.
+  intros n sq d e1 e2 H.
+  simpl in H.
+  tauto.
+Qed.
+
+Lemma trace_boolish_le_node_Mul :
+  forall n (sq : Vector.t Q n) (d : Q) (e1 e2 : GA_expr n),
+    trace_boolish_le sq (Mul e1 e2) d ->
+    boolish_le (mv_gp sq (eval_expr sq e1) (eval_expr sq e2)) d.
+Proof.
+  intros n sq d e1 e2 H.
+  simpl in H.
+  tauto.
+Qed.
+
+Lemma trace_boolish_le_node_Conv :
+  forall n (sq : Vector.t Q n) (d : Q) (e1 e2 : GA_expr n),
+    trace_boolish_le sq (Conv e1 e2) d ->
+    boolish_le (mv_conv (eval_expr sq e1) (eval_expr sq e2)) d.
+Proof.
+  intros n sq d e1 e2 H.
+  simpl in H.
+  tauto.
+Qed.
+
+Lemma computes_implies_final_boolish_0 :
+  forall n (sq : Vector.t Q n) (e : GA_expr n) (f : Corner n -> bool),
+    computes sq e f ->
+    boolish_le (eval_expr sq e) 0.
+Proof.
+  intros n sq e f Hcomp.
+  unfold boolish_le.
+  exists f.
+  (* dist_to is definitional equal to bool_dist_wrt, so the lemma gives equality *)
+  assert (Hz : bool_dist_wrt (eval_expr sq e) f == 0).
+  { exact (computes_implies_final_booldist_zero (n:=n) (sq:=sq) (e:=e) (f:=f) Hcomp). }
+  (* equality implies <= *)
+  apply (Qle_trans _ 0).
+  - apply Qle_of_Qeq. exact Hz.
+  - apply Qle_refl.
+Qed.
+
+Record EasyCompiler := {
+  R : nat -> Type;
+
+  target : forall {n : nat}, R n -> Corner n -> bool;
+  compile : forall {n : nat}, R n -> GA_expr n;
+
+  B : nat -> ExcNum;
+  d0 : Q;
+
+  compile_correct :
+    forall {n : nat} (sq : Vector.t Q n) (r : R n),
+      computes sq (compile (n:=n) r) (target (n:=n) r);
+
+  compile_exc_bound :
+    forall {n : nat} (sq : Vector.t Q n) (r : R n),
+      exc_pre (exc_of sq (compile (n:=n) r)) (B (expr_size (compile (n:=n) r)));
+
+  compile_boolish_bound :
+    forall {n : nat} (sq : Vector.t Q n) (r : R n),
+      trace_boolish_le sq (compile (n:=n) r) d0
+}.
+
+Definition compile' (C : EasyCompiler) {n} (r : R C n) : GA_expr n :=
+  compile C (n:=n) r.
+
+Definition target' (C : EasyCompiler) {n} (r : R C n) : Corner n -> bool :=
+  target C (n:=n) r.
+
+(*
+    those compile' and target' definitions allow
+      computes sq (compile' C r) (target' C r)
+*)
+
+
+(* Definition easy (C : EasyCompiler) {n} (f : Corner n -> bool) : Prop :=
+  exists r : R C n, forall x, target' C r x = f x. *)
+Definition easy (C : EasyCompiler) {n} (f : Corner n -> bool) : Prop :=
+  exists r : R C n, forall m : Mask n, embed (target' C r) m == embed f m.
+
+Lemma easy_implies_easy_under :
+  forall (C : EasyCompiler) n (sq : Vector.t Q n) (f : Corner n -> bool),
+    easy C (n:=n) f ->
+    easy_under (B C) (d0 C) sq f.
+Proof.
+  intros C n sq f [r Htgt_embed].
+  exists (compile' C r).
+  split.
+  - (* computes *)
+    intros m.
+    specialize (compile_correct C (n:=n) sq r) as Hcomp.
+    specialize (Hcomp m).
+    (* Hcomp: eval_expr sq (compile' C r) m == embed (target' C r) m *)
+    (* rewrite RHS using Htgt_embed *)
+    eapply Qeq_trans; [exact Hcomp |].
+    exact (Htgt_embed m).
+  - split.
+    + apply compile_exc_bound.
+    + apply compile_boolish_bound.
+Qed.
+
+Definition poly_B (k : nat) : nat -> ExcNum :=
+  fun s => {| exc_grade := s^k; exc_l1 := inject_Z (Z.of_nat (s^k)) |}.
+
+Fixpoint lincomb_embed {n}
+  (cs : list Q) (gs : list (Corner n -> bool)) : MV n :=
+  match cs, gs with
+  | [], [] => mv_zero
+  | c :: cs', g :: gs' =>
+      mv_add (mv_scale c (embed g)) (lincomb_embed cs' gs')
+  | _, _ => mv_zero (* or any default; enforce equal lengths in proofs *)
+  end.
+
+Definition wf_lincomb {n} (cs : list Q) (gs : list (Corner n -> bool)) : Prop :=
+  length cs = length gs.
+
+Definition boolish_k_le {n} (F : MV n) (k : nat) (d : Q) : Prop :=
+  exists (cs : list Q) (gs : list (Corner n -> bool)),
+    wf_lincomb cs gs /\
+    (length gs <= k)%nat /\
+    l1_norm (mv_sub F (lincomb_embed cs gs)) <= d.
+
+Lemma boolish_k_le_add :
+  forall n (F G : MV n) k1 k2 d1 d2,
+    boolish_k_le F k1 d1 ->
+    boolish_k_le G k2 d2 ->
+    boolish_k_le (mv_add F G) (k1 + k2) (d1 + d2).
+Proof.
+Admitted.
+
+Theorem all_easy_are_easy_under :
+  forall (C : EasyCompiler) n (sq : Vector.t Q n) (f : Corner n -> bool),
+    easy C (n:=n) f ->
+    easy_under (B C) (d0 C) sq f.
+Proof.
+  intros C n sq f Heasy.
+  exact (@easy_implies_easy_under C n sq f Heasy).
+Qed.
+
+Lemma mv_add_apply :
+  forall n (F G : MV n) (m : Mask n),
+    (F ⊕ G) m == F m + G m.
+Proof. reflexivity. Qed.
+
+Lemma lincomb_embed_app :
+  forall (n : nat)
+         (cs1 cs2 : list Q)
+         (gs1 gs2 : list (Corner n -> bool)),
+    wf_lincomb cs1 gs1 ->
+    wf_lincomb cs2 gs2 ->
+    forall m : Mask n,
+      lincomb_embed (cs1 ++ cs2) (gs1 ++ gs2) m
+      == mv_add (lincomb_embed cs1 gs1) (lincomb_embed cs2 gs2) m.
+Proof.
+  intros n cs1 cs2 gs1 gs2 Hwf1 Hwf2 m.
+  revert gs1 Hwf1 m.
+  induction cs1 as [|c cs1 IH]; intros gs1 Hwf1 m; simpl in *.
+  -
+    destruct gs1 as [|g gs1]; simpl in *.
+    + unfold mv_add, mv_zero; ring.
+    +
+      discriminate.
+  -
+    destruct gs1 as [|g gs1]; simpl in *.
+    + discriminate.
+    +
+      specialize (IH gs1).
+      assert (Hwf1' : wf_lincomb cs1 gs1).
+      { unfold wf_lincomb in *; simpl in *; lia. }
+      specialize (IH Hwf1' m).
+      unfold mv_add, mv_scale; simpl.
+      rewrite IH.
+      rewrite mv_add_apply.
+      rewrite Qplus_assoc.
+      reflexivity.
+Qed.
+
+Theorem hard_family_separates :
+  exists f : forall n, Corner n -> bool,
+  exists c > 0,
+  forall n sq e,
+    computes sq e (f n) ->
+    trace_boolish_le sq e d ->
+    exc_l1 (exc_of sq e) >= 2^(c*n).
+Proof.
+Admitted.
