Coq/Cln/TraceGeometry/open_rocqide.bat
@@ -1,0 +1,1 @@
+cd E:\GLogic\Coq\Cln\TraceGeometry & "C:\Rocq-Platform~9.0~2025.08\bin\rocqide.exe"
